# Bike Model
- Original differential EOMs
	- $T = I\alpha$
	- $F = ma$
- Transformed differential EOMs
	- $N = I_{z} \frac{dr}{dt}$
	- $Y = ma_y$
- $a_{y} = Vr + \dot{v} = Vr + V\dot{\beta} = V(r+\dot{\beta})$
- $\alpha_{R} = \frac{v-br}{V} = \frac{v}{V}-\frac{br}{V} = \beta-\frac{br}{V}$
- $\alpha_{F} = \beta + \frac{ar}{V}-\delta$
- $Y_{F} = C_{F}\beta+C_{F}(\frac{ar}{V})-C_{F}\delta$
- $Y_{R} = C_{R}\beta-C_{R}(\frac{br}{V})$
- $Y = Y_{F}+Y_{R}$
- $N = N_{F}+N_{R} = Y_{F}a-Y_{R}b$
- $Y = Y_{\beta}\beta+Y_{r}r+Y_{\delta}\delta$
	- $Y_{\beta} = C_{F}+C_{R}$
	- $Y_{r}=\frac{1}{V}(aC_{F}-bC_{R})$
	- $Y_{\delta}=-C_F$
- $N=N_{\beta}\beta+N_{r}r+N_{\delta}\delta$
	- $N_{\beta}=aC_{F}-bC_{R}$
	- $N_{r}=\frac{1}{V}(a^{2}C_{F}+b^{2}C_{R})$
	- $N_{\delta}=-aC_{F}$
- Final EOMs
	- $I_{z}\dot{r}=N_{\beta}\beta+N_{r}r+N_{\delta}\delta$
	- $mV(r+\dot{\beta})=Y_{\beta}\beta+Y_{r}r+Y_{\delta}\delta$
- Steady-State Response
	- The EOMs turn into:
		- $mVr=Y_{\beta}\beta+Y_{r}r+Y_{\delta}\delta$
		- $0=N_{\beta}\beta+N_{r}r+N_{\delta}\delta$
	- Knowing that in a SS turn $r=\frac{V}{R}$ gives:
		- $-Y_{\delta}=Y_{\beta}+(VY_{r}-mV^{2})(\frac{1}{R})$
		- $-N_{\delta}=N_{\beta}+VN_{r}(\frac{1}{R})$
	- Solving the $N_\delta$ equation for beta and subbing into first equation gives:
		- J4d6$NbaqNjQWg9